Compose soundness and completeness instead of correctness

theories/Stlc/Instantiation.v
@@ -45,81 +45,128 @@ Import ctx.notations.
 
 Notation Assignment := (@env.Env nat (fun _ => Ty)).
 
-Class Inst (A : TYPE) (a : Type) : Type :=
-  inst : forall {w}, A w -> Assignment w -> a.
+Section Inst.
 
-#[export] Instance inst_list {A : TYPE} {a : Type} `{Inst A a} :
-  Inst (List A) (list a) :=
-  fun w xs ass => List.map (fun x => inst x ass) xs.
+  Class Inst (A : TYPE) (a : Type) : Type :=
+    inst : forall {w}, A w -> Assignment w -> a.
 
-#[export] Instance inst_const {A} :
-  Inst (Const A) A | 10 :=
-  fun Σ x ι => x.
+  #[export] Instance inst_list {A : TYPE} {a : Type} `{Inst A a} :
+    Inst (List A) (list a) :=
+    fun w xs ass => List.map (fun x => inst x ass) xs.
 
-#[export] Instance inst_unit :
-  Inst Unit unit :=
-  fun _ x ass => x.
+  #[export] Instance inst_const {A} :
+    Inst (Const A) A | 10 :=
+    fun Σ x ι => x.
 
-#[export] Instance inst_prod {AT BT A B} `{Inst AT A, Inst BT B} :
-  Inst (Prod AT BT) (A * B) :=
-  fun ass '(a , b) ι => (inst a ι, inst b ι).
+  #[export] Instance inst_unit :
+    Inst Unit unit :=
+    fun _ x ass => x.
 
-#[export] Instance inst_option {AT A} `{Inst AT A} :
-  Inst (Option AT) (option A) :=
-  fun w ma ass => option_map (fun a => inst a ass) ma.
+  #[export] Instance inst_prod {AT BT A B} `{Inst AT A, Inst BT B} :
+    Inst (Prod AT BT) (A * B) :=
+    fun ass '(a , b) ι => (inst a ι, inst b ι).
 
-#[export] Instance inst_ty : Inst Ṫy Ty :=
-  fix inst_ty {w} t ι :=
-    match t with
-    | ṫy.var αIn    => env.lookup ι αIn
-    | ṫy.bool       => ty.bool
-    | ṫy.func t1 t2 => ty.func (inst_ty t1 ι) (inst_ty t2 ι)
-    end.
+  #[export] Instance inst_option {AT A} `{Inst AT A} :
+    Inst (Option AT) (option A) :=
+    fun w ma ass => option_map (fun a => inst a ass) ma.
 
-#[export] Instance inst_env : Inst Ėnv Env :=
-  fun w Γ ι => base.fmap (fun t : Ṫy w => inst t ι) Γ.
+  #[export] Instance inst_ty : Inst Ṫy Ty :=
+    fix inst_ty {w} t ι :=
+      match t with
+      | ṫy.var αIn    => env.lookup ι αIn
+      | ṫy.bool       => ty.bool
+      | ṫy.func t1 t2 => ty.func (inst_ty t1 ι) (inst_ty t2 ι)
+      end.
 
-#[export] Instance inst_acc {Θ : ACC} :
-  forall w, Inst (Θ w) (Assignment w).
-Proof.
-  intros w0 w1 θ ι.
-  apply env.tabulate.
-  intros α αIn.
-  apply (inst (lk θ αIn) ι).
-Defined.
+  #[export] Instance inst_env : Inst Ėnv Env :=
+    fun w Γ ι => base.fmap (fun t : Ṫy w => inst t ι) Γ.
+
+  #[export] Instance inst_acc {Θ : ACC} :
+    forall w, Inst (Θ w) (Assignment w) :=
+    fun w0 w1 θ ι => env.tabulate (fun α αIn => inst (lk θ αIn) ι).
+End Inst.
 
 Section Lift.
   Import World.notations.
 
+  Class Lift (AT : TYPE) (A : Type) : Type :=
+    lift : A -> ⊢ʷ AT.
+
   (* Indexes a given ty by a world Σ *)
-  Fixpoint lift (t : Ty) : ⊢ʷ Ṫy :=
-    fun w =>
+  #[export] Instance lift_ty : Lift Ṫy Ty :=
+    fix lift_ty (t : Ty) w : Ṫy w :=
       match t with
       | ty.bool       => ṫy.bool
-      | ty.func t1 t2 => ṫy.func (lift t1 w) (lift t2 w)
+      | ty.func t1 t2 => ṫy.func (lift_ty t1 w) (lift_ty t2 w)
       end.
 
-  Definition liftEnv (E : Env) : ⊢ʷ Ėnv.
-  Proof.
-    intros w. revert E. unfold Ėnv. apply base.fmap.
-    intros t. apply (lift t).
-  Defined.
+  #[export] Instance lift_env : Lift Ėnv Env :=
+    fun E w => fmap (fun t => lift t w) E.
 
-  Lemma inst_lift (w : World) (t : Ty) (ι : Assignment w) :
-    inst (lift t w) ι = t.
-  Proof. Admitted.
-
-  Lemma inst_lift_env (w : World) (G : Env) (ι : Assignment w) :
-    inst (liftEnv G w) ι = G.
-  Proof. Admitted.
+  #[export] Instance lift_prod {AT BT A B} `{Lift AT A, Lift BT B} :
+    Lift (Prod AT BT) (A * B) :=
+    fun '(a , b) w => (lift a w, lift b w).
 
 End Lift.
 
-Lemma inst_persist {Θ : ACC}
-  {AT A} {pers : Persistent AT} {instAT : Inst AT A}
-  {w0 w1} (θ : Θ w0 w1) (t : AT w0) (ι : Assignment w1) :
-  inst (persist t θ) ι = inst t (inst θ ι).
-Proof. Admitted.
+Section InstLift.
+
+  Class InstLift AT A `{Inst AT A, Lift AT A} : Prop :=
+    inst_lift (w : World) (a : A) (ι : Assignment w) :
+      inst (lift a w) ι = a.
+  #[global] Arguments InstLift _ _ {_ _}.
+
+  #[export] Instance inst_lift_ty : InstLift Ṫy Ty.
+  Proof. intros w t ι. induction t; cbn; f_equal; auto. Qed.
+
+  #[export] Instance inst_lift_env : InstLift Ėnv Env.
+  Proof.
+    intros w E ι. unfold inst, inst_env, lift, lift_env.
+    rewrite <- map_fmap_id. rewrite <- map_fmap_compose.
+    apply map_fmap_ext. intros x t Hlk. apply inst_lift.
+  Qed.
+
+End InstLift.
+
+Section InstPersist.
+
+  Class InstPersist AT A `{Persistent AT, Inst AT A} : Prop :=
+    inst_persist [Θ : ACC] {w0 w1} (θ : Θ w0 w1) (t : AT w0) (ι : Assignment w1) :
+      inst (persist t θ) ι = inst t (inst θ ι).
+  #[global] Arguments InstPersist _ _ {_ _}.
+
+  #[export] Instance inst_persist_ty : InstPersist Ṫy Ty.
+  Proof.
+    intros Θ w0 w1 θ t ι. induction t; cbn; f_equal; auto.
+    unfold inst at 2, inst_acc. now rewrite env.lookup_tabulate.
+  Qed.
+
+  #[export] Instance inst_persist_env : InstPersist Ėnv Env.
+  Proof.
+    intros Θ w0 w1 θ E ι. unfold persist, persist_env, inst at 1 2, inst_env.
+    rewrite <- map_fmap_compose. apply map_fmap_ext.
+    intros x t Hlk. apply inst_persist.
+  Qed.
+
+End InstPersist.
+
+Section PersistLift.
+  Class PersistLift AT A {liftA : Lift AT A} {persA: Persistent AT} : Prop :=
+    persist_lift [Θ : ACC] {w0 w1} (a : A) (θ : Θ w0 w1) :
+      persist (lift a w0) θ = lift a w1.
+  #[global] Arguments PersistLift _ _ {_ _}.
+
+  #[export] Instance persist_lift_ty : PersistLift Ṫy Ty.
+  Proof. intros Θ w0 w1 t θ. induction t; cbn; f_equal; auto. Qed.
+
+  #[export] Instance persist_lift_env : PersistLift Ėnv Env.
+  Proof.
+    intros Θ w0 w1 E θ. unfold persist, lift, persist_env, lift_env, Ėnv.
+    rewrite <- map_fmap_compose. apply map_fmap_ext.
+    intros x t Hlk. apply persist_lift.
+  Qed.
+
+End PersistLift.
 
 Lemma inst_refl {Θ} {reflΘ : Refl Θ} {lkreflΘ : LkRefl Θ} :
   forall w (ι : Assignment w), inst (refl (Θ := Θ)) ι = ι.
@@ -136,30 +183,46 @@ Proof.
   now rewrite ?env.lookup_tabulate, lk_trans, inst_persist.
 Qed.
 
-Lemma inst_reduce {Θ} {reduceΘ : Reduce Θ} :
-  forall {w α t} (ι : Assignment w),
-    inst (reduce α t) ι = env.snoc ι α (inst t ι).
-Proof. Admitted.
+Lemma inst_reduce {Θ} {reduceΘ : Reduce Θ} {w α t} (ι : Assignment w) :
+  inst (reduce α t) ι = env.snoc ι α (inst t ι).
+Proof.
+  apply env.lookup_extensional. intros β βIn. unfold inst, inst_acc.
+  rewrite env.lookup_tabulate. cbn.
+  destruct ctx.view; cbn.
+  - now rewrite lk_reduce_zero.
+  - now rewrite lk_reduce_succ.
+Qed.
 
-Lemma inst_step {Θ} {stepΘ : Step Θ} :
-  forall {w x} (ι : Assignment (w ▻ x)),
-    inst (step (Θ := Θ)) ι = let (ι',_) := env.view ι in ι'.
-Proof. Admitted.
+Lemma inst_step_snoc {Θ} {stepΘ : Step Θ} {w x} (ι : Assignment w) (t : Ty) :
+  inst (step (Θ := Θ)) (env.snoc ι x t) = ι.
+Proof.
+  apply env.lookup_extensional. intros α αIn. unfold inst, inst_acc.
+  rewrite env.lookup_tabulate. rewrite lk_step. reflexivity.
+Qed.
 
-Lemma inst_step_snoc {Θ} {stepΘ : Step Θ} :
-  forall {w x} (ι : Assignment w) (t : Ty),
-    inst (step (Θ := Θ)) (env.snoc ι x t) = ι.
-Proof. intros. rewrite inst_step. reflexivity. Qed.
+Lemma inst_step {Θ} {stepΘ : Step Θ} {w x} (ι : Assignment (w ▻ x)) :
+  inst (step (Θ := Θ)) ι = let (ι',_) := env.view ι in ι'.
+Proof. destruct env.view. apply inst_step_snoc. Qed.
 
 Lemma inst_thin {Θ} {thinΘ : Thin Θ}
   {w} (ι : Assignment w) {α} (αIn : α ∈ w) :
   inst (thin α) ι = env.remove α ι αIn.
-Proof. Admitted.
+Proof.
+  apply env.lookup_extensional. intros β βIn. unfold inst, inst_acc.
+  rewrite env.lookup_tabulate. rewrite lk_thin. cbn.
+  now rewrite env.lookup_thin.
+Qed.
 
 Lemma inst_thick {Θ} {thickΘ : Thick Θ} :
   forall {w} {x} (xIn : x ∈ w) (t : Ṫy (w - x)) (ι : Assignment (w - x)),
-      inst (thick (Θ := Θ) x t) ι = env.insert xIn ι (inst t ι).
-Proof. Admitted.
+    inst (thick (Θ := Θ) x t) ι = env.insert xIn ι (inst t ι).
+Proof.
+  intros. apply env.lookup_extensional. intros β βIn. unfold inst, inst_acc.
+  rewrite env.lookup_tabulate. rewrite lk_thick. cbn. unfold thickIn.
+  destruct ctx.occurs_check_view; cbn.
+  - now rewrite env.lookup_insert.
+  - now rewrite env.lookup_thin, env.remove_insert.
+Qed.
 
 Lemma inst_direct_subterm {w} (t1 t2 : Ṫy w) (ι : Assignment w) :
   ṫy.Ṫy_direct_subterm t1 t2 ->
@@ -175,9 +238,9 @@ Proof.
 Qed.
 
 Lemma lookup_lift (Γ : Env) (x : string) (w : World) :
-  lookup x (liftEnv Γ w) =
+  lookup x (lift Γ w) =
     option.map (fun t => lift t w) (lookup x Γ).
-Proof. unfold liftEnv. now rewrite <- lookup_fmap. Qed.
+Proof. unfold lift, lift_env. now rewrite <- lookup_fmap. Qed.
 
 Lemma lookup_inst (w : World) (Γ : Ėnv w) (x : string) (ι : Assignment w) :
   lookup x (inst Γ ι) = inst (lookup x Γ) ι.
@@ -194,26 +257,22 @@ Lemma inst_empty {w} (ι : Assignment w) :
   inst (A := Ėnv) empty ι = empty.
 Proof. cbv [inst inst_env Ėnv]. now rewrite fmap_empty. Qed.
 
-Lemma liftEnv_insert {w x t Γ} :
-  liftEnv (insert x t Γ) w = insert x (lift t w) (liftEnv Γ w).
-Proof. unfold liftEnv. now rewrite fmap_insert. Qed.
-
-Lemma persist_liftTy {Θ : ACC} {w0 w1} t (θ : Θ w0 w1) :
-  persist (lift t w0) θ = lift t w1.
-Proof. induction t; cbn; f_equal; auto. Qed.
+Lemma lift_insert {w x t Γ} :
+  lift (insert x t Γ) w = insert x (lift t w) (lift Γ w).
+Proof. unfold lift, lift_env. now rewrite fmap_insert. Qed.
 
   (* Lemma persist_split : forall w w' iw (pos : w ↑ iw) (neg : iw ↓ w') x, *)
   (*   persist w  x iw pos -> *)
   (*   persist iw x w' neg -> *)
   (*   persist w  x w' {| iw := iw; pos := pos; neg := neg |}. *)
 
-Lemma persist_liftEnv {Θ : ACC} {w0 w1} (e : Env) (θ : Θ w0 w1) :
-  persist (liftEnv e w0) θ = liftEnv e w1.
-Proof.
-  unfold liftEnv, persist, persist_env. rewrite <- map_fmap_compose.
-  apply (map_fmap_ext (M := gmap string)). intros _ t _.
-  unfold compose. apply persist_liftTy.
-Qed.
+(* Lemma persist_liftEnv {Θ : ACC} {w0 w1} (e : Env) (θ : Θ w0 w1) : *)
+(*   persist (liftEnv e w0) θ = liftEnv e w1. *)
+(* Proof. *)
+(*   unfold liftEnv, persist, persist_env. rewrite <- map_fmap_compose. *)
+(*   apply (map_fmap_ext (M := gmap string)). intros _ t _. *)
+(*   unfold compose. apply persist_liftTy. *)
+(* Qed. *)
 
 Fixpoint grounding (w : World) : Assignment w :=
   match w with
