theories/Stlc/Substitution.v
@@ -270,15 +270,27 @@ Module Sub.
 
   Lemma of_step {Θ} {stepΘ : Step Θ} w α :
     of (@step Θ stepΘ w α) = step (Θ := Sub).
-  Proof. Admitted.
+  Proof.
+    apply env.lookup_extensional. intros β βIn. unfold of. cbn.
+    rewrite !env.lookup_tabulate. now rewrite lk_step.
+  Qed.
 
   Lemma of_reduce {Θ} {reduceΘ : Reduce Θ} w α t :
     of (@reduce Θ reduceΘ w α t) = reduce (Θ := Sub) α t.
-  Proof. Admitted.
+  Proof.
+    apply env.lookup_extensional. intros β βIn. unfold of.
+    rewrite env.lookup_tabulate. cbn.
+    destruct ctx.view.
+    - now rewrite lk_reduce_zero.
+    - rewrite lk_reduce_succ. symmetry. apply (lk_refl (Θ := Sub)).
+  Qed.
 
   Lemma of_thick {Θ} {thickΘ : Thick Θ} w α αIn t :
     of (@thick Θ thickΘ w α αIn t) = thick (Θ := Sub) α t.
-  Proof. Admitted.
+  Proof.
+    apply env.lookup_extensional. intros β βIn. unfold of, thick at 2, thick_sub.
+    now rewrite !env.lookup_tabulate, lk_thick.
+  Qed.
 
   Lemma of_trans {Θ} {transΘ : Trans Θ} {lktransΘ : LkTrans Θ}
     {w0 w1 w2} (θ1 : Θ w0 w1) (θ2 : Θ w1 w2) :
