flake.nix
@@ -1,0 +1,55 @@
+{
+  inputs.nixpkgs.url = "github:NixOS/nixpkgs/nixos-unstable";
+  inputs.flake-utils.url = "github:numtide/flake-utils";
+
+  outputs = inputs:
+    inputs.flake-utils.lib.eachDefaultSystem (
+      system: let
+        pkgs = import inputs.nixpkgs {inherit system;};
+        # Function to override versions of coq packages. This function takes two arguments:
+        # - coqPackages: The set of all Coq packages.
+        # - versions: An attribute set of packages with their versions we want to override.
+        patchCoqPackages = coqPackages: versions:
+          coqPackages.overrideScope' (
+            _self: super:
+              pkgs.lib.foldlAttrs
+              # foldAttrs is used to iterate over the versions set and apply a function
+              # to each attribute. This function takes three arguments: the accumulator set,
+              # the attribute name (package name), and the attribute value (version).
+              (acc: pkg: version:
+                # This function returns a new set with the current attribute added to the
+                # accumulator set. The attribute name is the package name, and the value
+                # is the overridden package.
+                  acc // {${pkg} = super.${pkg}.override {inherit version;};})
+              # The initial value of the accumulator set.
+              {}
+              # The attribute set to iterate over.
+              versions
+          );
+
+        iris40 = {
+          iris = "4.0.0";
+          stdpp = "1.8.0";
+        };
+
+        coqPackages816 = with (patchCoqPackages pkgs.coqPackages_8_16 iris40); [coq equations stdpp iris];
+        coqPackages817 = with (patchCoqPackages pkgs.coqPackages_8_17 iris40); [coq equations stdpp iris];
+
+        emacsPackage = (pkgs.emacsPackagesFor pkgs.emacs).emacsWithPackages (ep:
+          with ep; [
+            company-coq
+            magit
+            proof-general
+          ]);
+      in {
+        devShells = rec {
+          default = coq817;
+          coq816 = pkgs.mkShell {buildInputs = coqPackages816;};
+          coq817 = pkgs.mkShell {buildInputs = coqPackages817;};
+
+          emacs816 = pkgs.mkShell {buildInputs = coqPackages816 ++ [emacsPackage];};
+          emacs817 = pkgs.mkShell {buildInputs = coqPackages817 ++ [emacsPackage];};
+        };
+      }
+    );
+}
